Fix linking

vale/code/arch/x64/interop/GCMencryptOpt_stdcalls.fst
@@ -12,7 +12,191 @@ open FStar.Calc
 
 let math_aux (n:nat) : Lemma (n * 1 == n) = ()
 
-let gcm128_encrypt key auth_b auth_bytes auth_num keys_b iv_b hkeys_b abytes_b
+
+inline_for_extraction
+val gcm128_encrypt_opt':
+  key:Ghost.erased (Seq.seq nat32) ->
+  auth_b:uint8_p ->
+  auth_bytes:uint64 ->
+  auth_num:uint64 ->
+  keys_b:uint8_p ->
+  iv_b:uint8_p ->
+  hkeys_b:uint8_p ->
+  abytes_b:uint8_p ->
+  in128x6_b:uint8_p ->
+  out128x6_b:uint8_p ->
+  len128x6:uint64 ->
+  in128_b:uint8_p ->
+  out128_b:uint8_p ->
+  len128_num:uint64 ->
+  inout_b:uint8_p ->
+  plain_num:uint64 ->
+
+  scratch_b:uint8_p ->
+  tag_b:uint8_p ->
+
+  Stack unit
+    (requires fun h0 ->
+      B.disjoint tag_b out128x6_b /\ B.disjoint tag_b out128_b /\
+      B.disjoint tag_b inout_b /\ B.disjoint tag_b hkeys_b /\
+      disjoint_or_eq tag_b auth_b /\ disjoint_or_eq tag_b iv_b /\
+      disjoint_or_eq tag_b keys_b /\ disjoint_or_eq tag_b abytes_b /\
+      disjoint_or_eq tag_b in128x6_b /\ disjoint_or_eq tag_b in128_b /\
+      disjoint_or_eq tag_b scratch_b /\
+
+      B.disjoint iv_b keys_b /\ B.disjoint iv_b scratch_b /\ B.disjoint iv_b in128x6_b /\
+      B.disjoint iv_b out128x6_b /\ B.disjoint iv_b hkeys_b /\ B.disjoint iv_b in128_b /\
+      B.disjoint iv_b out128_b /\ B.disjoint iv_b inout_b /\
+      disjoint_or_eq iv_b auth_b /\ disjoint_or_eq iv_b abytes_b /\
+
+      B.disjoint scratch_b keys_b /\ B.disjoint scratch_b in128x6_b /\
+      B.disjoint scratch_b out128x6_b /\ B.disjoint scratch_b in128_b /\
+      B.disjoint scratch_b out128_b /\ B.disjoint scratch_b inout_b /\
+      B.disjoint scratch_b hkeys_b /\
+      disjoint_or_eq scratch_b auth_b /\ disjoint_or_eq scratch_b abytes_b /\
+
+      B.disjoint out128x6_b keys_b /\ B.disjoint out128x6_b hkeys_b /\
+      B.disjoint out128x6_b in128_b /\ B.disjoint out128x6_b inout_b /\
+      B.disjoint out128x6_b out128_b /\
+      disjoint_or_eq out128x6_b in128x6_b /\
+      disjoint_or_eq out128x6_b auth_b /\ disjoint_or_eq out128x6_b abytes_b /\
+
+      B.disjoint out128_b keys_b /\ B.disjoint out128_b hkeys_b /\
+      B.disjoint out128_b inout_b /\
+      disjoint_or_eq out128_b in128_b /\ disjoint_or_eq out128_b in128x6_b /\
+      disjoint_or_eq out128_b auth_b /\ disjoint_or_eq out128_b abytes_b /\
+
+      B.disjoint inout_b keys_b /\ B.disjoint inout_b hkeys_b /\
+      disjoint_or_eq inout_b in128_b /\ disjoint_or_eq inout_b in128x6_b /\
+      disjoint_or_eq inout_b auth_b /\ disjoint_or_eq inout_b abytes_b /\
+
+      disjoint_or_eq keys_b hkeys_b /\ 
+      disjoint_or_eq keys_b in128x6_b /\ disjoint_or_eq keys_b in128_b /\
+      disjoint_or_eq keys_b auth_b /\ disjoint_or_eq keys_b abytes_b /\
+
+      disjoint_or_eq hkeys_b in128_b /\ disjoint_or_eq hkeys_b in128x6_b /\
+      disjoint_or_eq hkeys_b auth_b /\ disjoint_or_eq hkeys_b abytes_b /\
+
+      disjoint_or_eq in128_b in128x6_b /\ disjoint_or_eq in128_b auth_b /\
+      disjoint_or_eq in128_b abytes_b /\
+      
+      disjoint_or_eq in128x6_b auth_b /\ disjoint_or_eq in128x6_b abytes_b /\
+      
+      disjoint_or_eq auth_b abytes_b /\
+
+      B.live h0 auth_b /\ B.live h0 abytes_b /\ B.live h0 keys_b /\
+      B.live h0 iv_b /\ B.live h0 hkeys_b /\
+      B.live h0 in128x6_b /\ B.live h0 out128x6_b /\
+      B.live h0 in128_b /\ B.live h0 out128_b /\
+      B.live h0 inout_b /\ B.live h0 tag_b /\ B.live h0 scratch_b /\
+
+      B.length auth_b = 16 * UInt64.v auth_num /\
+      B.length abytes_b == 16 /\
+      B.length iv_b = 16 /\
+      B.length in128x6_b == 16 * UInt64.v len128x6 /\
+      B.length out128x6_b == B.length in128x6_b /\
+      B.length in128_b == 16 * UInt64.v len128_num /\
+      B.length out128_b == B.length in128_b /\
+      B.length inout_b == 16 /\
+      B.length scratch_b == 128 /\
+      B.length hkeys_b = 160 /\
+      B.length tag_b == 16 /\
+      B.length keys_b = 176 /\
+
+      8 * (UInt64.v plain_num) < pow2_32 /\
+      4096 * 16 * (UInt64.v len128x6) < pow2_32 /\
+      4096 * (UInt64.v len128_num) < pow2_32 /\
+      4096 * (UInt64.v auth_bytes) < pow2_32 /\
+
+      UInt64.v len128x6 % 6 == 0 /\
+      UInt64.v len128x6 >= 18 /\
+      12 + UInt64.v len128x6 + 6 < pow2_32 /\
+
+      aesni_enabled /\ pclmulqdq_enabled /\
+      is_aes_key_LE AES_128 (Ghost.reveal key) /\
+      (let db = get_downview keys_b in
+      length_aux keys_b;
+      let ub = UV.mk_buffer db Views.up_view128 in
+      Seq.equal (UV.as_seq h0 ub) (key_to_round_keys_LE AES_128 (Ghost.reveal key)))
+    )
+    (ensures fun h0 _ h1 ->
+      B.modifies (B.loc_union (B.loc_buffer tag_b)
+                  (B.loc_union (B.loc_buffer iv_b)
+                  (B.loc_union (B.loc_buffer scratch_b)
+                  (B.loc_union (B.loc_buffer out128x6_b)
+                  (B.loc_union (B.loc_buffer out128_b)
+                  (B.loc_buffer inout_b)))))) h0 h1 /\
+      (8 * (UInt64.v plain_num) < pow2_32 /\
+       8 * (UInt64.v auth_bytes) < pow2_32 /\ (
+       let in128x6_d = get_downview in128x6_b in
+       length_aux3 in128x6_b (UInt64.v len128x6);
+       let in128x6_u = UV.mk_buffer in128x6_d Views.up_view128 in
+       let in128_d = get_downview in128_b in
+       length_aux3 in128_b (UInt64.v len128_num);
+       let in128_u = UV.mk_buffer in128_d Views.up_view128 in
+       let inout_d = get_downview inout_b in
+       length_aux3 inout_b 1;      
+       let inout_u = UV.mk_buffer inout_d Views.up_view128 in       
+       let out128x6_d = get_downview out128x6_b in
+       length_aux3 out128x6_b (UInt64.v len128x6);
+       let out128x6_u = UV.mk_buffer out128x6_d Views.up_view128 in
+       let out128_d = get_downview out128_b in
+       length_aux3 out128_b (UInt64.v len128_num);
+       let out128_u = UV.mk_buffer out128_d Views.up_view128 in       
+       length_aux4 iv_b;
+       DV.length_eq (get_downview iv_b);
+       let iv_LE = low_buffer_read TUInt8 TUInt128 h0 iv_b 0 in
+       let iv_BE = reverse_bytes_quad32 iv_LE in
+       let ctr_BE_1 = Mkfour 1 iv_BE.lo1 iv_BE.hi2 iv_BE.hi3 in
+       let ctr_BE_2 = Mkfour 2 iv_BE.lo1 iv_BE.hi2 iv_BE.hi3 in
+       let plain_in =
+         if (UInt64.v plain_num > (UInt64.v len128x6 + UInt64.v len128_num) * 128/8) then
+           Seq.append (Seq.append (UV.as_seq h0 in128x6_u) (UV.as_seq h0 in128_u))
+                      (UV.as_seq h0 inout_u)
+         else Seq.append (UV.as_seq h0 in128x6_u) (UV.as_seq h0 in128_u)
+       in let cipher_out =
+         if (UInt64.v plain_num > (UInt64.v len128x6 + UInt64.v len128_num) * 128/8) then
+           Seq.append (Seq.append (UV.as_seq h1 out128x6_u) (UV.as_seq h1 out128_u))
+                      (UV.as_seq h1 inout_u)
+         else Seq.append (UV.as_seq h1 out128x6_u) (UV.as_seq h1 out128_u)
+       in gctr_partial AES_128 (UInt64.v len128x6 + UInt64.v len128_num + 1) plain_in cipher_out (Ghost.reveal key) ctr_BE_2 /\ (
+       DV.length_eq (get_downview hkeys_b);
+       let h = reverse_bytes_quad32 (low_buffer_read TUInt8 TUInt128 h1 hkeys_b 0) in
+       let length_quad = reverse_bytes_quad32 (Mkfour (8 * UInt64.v plain_num) 0 (8 * UInt64.v auth_bytes) 0) in
+       let auth_d = get_downview auth_b in
+       length_aux3 auth_b (UInt64.v auth_num);
+       let auth_u = UV.mk_buffer auth_d Views.up_view128 in
+       let abytes_d = get_downview abytes_b in
+       length_aux3 abytes_b 1;      
+       let abytes_u = UV.mk_buffer abytes_d Views.up_view128 in        
+       let cipher_bytes =
+         if UInt64.v plain_num > (UInt64.v len128x6 + UInt64.v len128_num) * 128/8 then
+           UV.as_seq h1 inout_u
+         else Seq.empty
+       in let auth_in =
+         if UInt64.v auth_bytes > UInt64.v auth_num * 128 / 8 then
+           Seq.append (Seq.append (Seq.append (Seq.append (Seq.append
+             (UV.as_seq h0 auth_u) (UV.as_seq h0 abytes_u))
+             (UV.as_seq h1 out128x6_u))
+             (UV.as_seq h1 out128_u))
+             cipher_bytes)
+             (Seq.create 1 length_quad)
+         else
+           Seq.append (Seq.append (Seq.append (Seq.append
+             (UV.as_seq h0 auth_u) (UV.as_seq h1 out128x6_u))
+             (UV.as_seq h1 out128_u))
+             cipher_bytes)
+             (Seq.create 1 length_quad)
+       in
+       DV.length_eq (get_downview tag_b);
+       low_buffer_read TUInt8 TUInt128 h1 tag_b 0 ==
+         gctr_encrypt_block ctr_BE_1 (ghash_LE h auth_in) AES_128 (Ghost.reveal key) 0
+         )
+         ))
+    )
+
+
+let gcm128_encrypt_opt' key auth_b auth_bytes auth_num keys_b iv_b hkeys_b abytes_b
   in128x6_b out128x6_b len128x6 in128_b out128_b len128_num inout_b plain_num scratch_b tag_b =
   
   let h0 = get() in
@@ -85,9 +269,9 @@ let gcm128_encrypt key auth_b auth_bytes auth_num keys_b iv_b hkeys_b abytes_b
 
   let h1 = get() in
   ()
-  // gcm_simplify1 plain_b h0 (UInt64.v plain_num);
-  // gcm_simplify1 auth_b h0 (UInt64.v auth_num);
-  // gcm_simplify1 out_b h1 (UInt64.v plain_num);
-  // gcm_simplify2 tag_b h1;
-  // gcm_simplify3 iv_b h0
 
+let gcm128_encrypt_opt_stdcall key plain_b plain_len auth_b auth_len iv_b out_b tag_b keys_b hkeys_b =
+  push_frame();
+  let scratch_b = B.alloca 0uy 128ul in
+  admit();
+  pop_frame()
