providers/evercrypt/EverCrypt.Vale.fsti
@@ -31,7 +31,7 @@ val old_aes128_key_expansion: key_ptr:uint8_p -> expanded_key_ptr: uint8_p -> St
 val old_gcm128_encrypt: B.pointer gcm_args -> Stack_ unit
 
 [@ (CCConv "stdcall") ]
-val old_gcm128_decrypt: B.pointer gcm_args -> Stack_ uint32_t
+val gcm128_decrypt: B.pointer gcm_args -> Stack_ uint32_t
 
 [@ (CCConv "stdcall") ]
 val old_aes256_key_expansion: key_ptr:uint8_p -> expanded_key_ptr: uint8_p -> Stack_ unit
@@ -40,4 +40,4 @@ val old_aes256_key_expansion: key_ptr:uint8_p -> expanded_key_ptr: uint8_p -> St
 val old_gcm256_encrypt: B.pointer gcm_args -> Stack_ unit
 
 [@ (CCConv "stdcall") ]
-val old_gcm256_decrypt: B.pointer gcm_args -> Stack_ uint32_t
+val gcm256_decrypt: B.pointer gcm_args -> Stack_ uint32_t
